HMAC: Update on the assumed SHA2 incremental pure specification

crypto_hst/hmac/Hash.Sha256.Pure.fst
@@ -1,13 +1,21 @@
 module Hash.Sha256.Pure
 
-open Hacl.UInt32
-open Hacl.SBuffer
+module U8 = FStar.UInt8
+module S8 = Hacl.UInt8
+module U32 = FStar.UInt32
+module S32 = Hacl.UInt32
+module U64 = FStar.UInt64
+module S64 = Hacl.UInt64
+module SB = Hacl.SBuffer
 
 
 (* Define base types *)
+let u8 = FStar.UInt8.t
+let s8 = Hacl.UInt8.t
 let u32 = FStar.UInt32.t
-let uint32s = Hacl.SBuffer.u32s
-let bytes = Seq.seq Hacl.UInt8.t
+let s32 = Hacl.UInt32.t
+let uint32s = Seq.seq s32
+let bytes = Seq.seq s8
 
 
 (* Define algorithm parameters *)
@@ -18,15 +26,14 @@ let blocksize = bl
 
 
 (* Define SHA2 functions *)
-(*
+
 assume val init : unit -> Tot (state:uint32s)
 
-assume val update : (state:uint32s) -> (data:bytes) -> (len:u32{length data = v len})
+assume val update : (state:uint32s) -> (data:bytes) -> (len:s32{Seq.length data = S32.v len})
   -> Tot (state :uint32s)
 
 assume val finish : (state:uint32s)
-  -> Tot (Prims.tuple2 (hash:bytes{length hash = v hashsize}) (state:uint32s))
-*)
+  -> Tot (Prims.tuple2 (hash:bytes{Seq.length hash = U32.v hashsize}) (state:uint32s))
 
-assume val sha256 : (data:bytes) -> (len:u32{Seq.length data = v len})
-  -> Tot (hash:bytes{Seq.length hash = v hashsize})
+assume val sha256 : (data:bytes) -> (len:s32{Seq.length data = S32.v len})
+  -> Tot (hash:bytes{Seq.length hash = U32.v hashsize})
